pulse/lib/pulse/lib/pledge/Pulse.Lib.InvList.fsti
@@ -18,7 +18,7 @@ module Pulse.Lib.InvList
 
 open Pulse.Lib.Pervasives
 
-let invlist_elem = storable & iname
+let invlist_elem = slprop & iname
 let invlist0 = list invlist_elem
 
 let rec invlist_names (is : invlist0) : inames =
@@ -56,7 +56,7 @@ val dup_invlist_inv (is:invlist)
 
 val shift_invlist_one
   (#a:Type0)
-  (p : storable)
+  (p : slprop)
   (i : iname)
   (is : invlist{not (mem_inv (invlist_names is) i)})
   (#pre:slprop)
@@ -68,7 +68,7 @@ val shift_invlist_one
 val with_invlist (#a:Type0) (#pre : slprop) (#post : a -> slprop)
   (is : invlist)
   (f : unit -> stt_ghost a emp_inames (invlist_v is ** pre) (fun v -> invlist_v is ** post v))
-  : stt_ghost a (invlist_names is) (invlist_inv is ** pre) (fun v -> invlist_inv is ** post v)
+  : stt_ghost a (invlist_names is) (invlist_inv is ** pre ** later_credit (List.Tot.length is)) (fun v -> invlist_inv is ** post v)
 
 (* A helper for a ghost-unit function. *)
 // val with_invlist_ghost (#pre : slprop) (#post : slprop)
